Try to get rid of the admits in Shared. Not possible.

io/case-studies/Shared.fst
@@ -28,13 +28,17 @@ let rec is_open (fd:file_descr) (h: trace) : Tot bool =
                  else is_open fd tail
                | _ -> is_open fd tail
 
-let ctx_pre (fd:file_descr) (h:trace) : Type0 = True 
+let ctx_pre (fd:file_descr) (h:trace) : Type0 = True
 
+
+(** The post-condition is too storng to be able to write a monitorable prop (pi).
+   The problem is that we can not prevent with the pi the closing of a file_descr by the 
+   plugin **)
 let ctx_post : file_descr -> trace -> r:(maybe unit) -> trace -> Tot (b:bool{r == Inr Contract_failure ==> b == true}) = 
   fun fd h r lt -> 
     match r with
     | Inr Contract_failure -> true
-    | _ -> is_open fd (apply_changes h lt)
+    | _ -> not (is_open fd h) || is_open fd (apply_changes h lt)
 
 
 val pi : monitorable_prop
@@ -44,10 +48,23 @@ let pi cmd arg h =
     let (fnm, _, _) : io_args Openfile = arg in not (fnm = "/etc/passwd")
   | _ -> true
 
+private
+let lemma_c1post_0 fd h lt :
+  Lemma
+    (requires (ctx_pre fd h /\ enforced_locally pi h lt))
+    (ensures (exists r. ctx_post fd h r lt)) = admit ()
+
+private
+let lemma_c1post () : squash (forall x h lt. ctx_pre x h /\ enforced_locally pi h lt ==> (exists r. ctx_post x h r lt)) = 
+  Classical.forall_intro_3 (Classical.move_requires_3 (lemma_c1post_0))
+
+private
+let lemma_c2post () : squash (forall x h r lt. ctx_pre x h /\ enforced_locally pi h lt  ==> ctx_post x h r lt) = admit ()
+
 instance ctx_post_monitorable () : monitorable_post ctx_pre (fun x h r lt -> ctx_post x h r lt) pi = {
   result_check = (fun _ _ _ _ -> true);
-  c1post = admit ();
-  c2post = ();
+  c1post = lemma_c1post ();
+  c2post = lemma_c2post ();
 }
 
 noeq type shared_interface = {
